# Deriving Equation (13)

The Lyapunov function $V(\vec{x})$ is defined as

$$
\begin{aligned}
    V(\vec{x}) &= \sum_{k = 1}^{n} \varepsilon_{k} |\vec{v}_{k}^{H} \vec{x}|^{2} \\
    &= \sum_{k = 1}^{n} \varepsilon_{k} \vec{x}^{H} \vec{v}_{k} \vec{v}_{k}^{H} \vec{x}
\end{aligned}
$$

Where $\varepsilon_{k}>0,k=0,1,\cdots,n$. $\vec{v}_{k}^{H}$ denotes the conjugate transpose of $\vec{v}_{k}$.

Then, we can obtain

$$
\begin{aligned}
    \dot{V}(\vec{x}) &= \sum_{k = 1}^{n} \varepsilon_{k} \frac{d}{dt} \Bigg(\vec{x}^{H} \vec{v}_{k} \vec{v}_{k}^{H} \vec{x} \Bigg) \\
    &= \sum_{k = 1}^{n} \varepsilon_{k} \frac{d \vec{x}^{\top}}{dt} \frac{d}{d \vec{x}} \Bigg(\vec{x}^{H} \vec{v}_{k} \vec{v}_{k}^{H} \vec{x} \Bigg) \\
    &= \sum_{k = 1}^{n} \varepsilon_{k} \frac{d \vec{x}^{\top}}{dt} \Bigg(2 \vec{v}_{k} \vec{v}_{k}^{H} \vec{x} \Bigg) \\
    &= \sum_{k = 1}^{n} 2 \varepsilon_{k} \vec{x}^{\top} A_{i}^{\top} (\vec{v}_{k} \vec{v}_{k}^{H} \vec{x})
\end{aligned}
$$
